Matroids/Verification/Count.lean
@@ -59,8 +59,8 @@ lemma forall_groupByValue (f : α → List ℕ) (A : List α) (hA : A.Forall P) 
 
 --
 
-lemma sort_join_sort {α :Type} [LinearOrder α] (L : List (List α)) :
-  List.sort (List.join (List.sort L)) = List.sort (List.join (L)) := by
+lemma sort_join_sort {X :Type} [LinearOrder X] (L : List (List X)) :
+    List.sort (List.join (List.sort L)) = List.sort (List.join (L)) := by
   match L with
   |[] => simp
   |a :: ll =>
@@ -74,13 +74,13 @@ lemma sort_join_sort {α :Type} [LinearOrder α] (L : List (List α)) :
       sorry
 -- proof idea: consider number of occurence in each list, should be the same
 
-lemma sort_join_map_sort (L : List (List Nat)) :
-  List.sort (List.join (List.map List.sort L)) = List.sort (List.join (L)) := by
+lemma sort_join_map_sort {X : Type} [LinearOrder X] (L : List (List X)):
+    List.sort (List.join (List.map List.sort L)) = List.sort (List.join (L)) := by
   sorry
 
 -- TODO generalize codomain of `f` to arbitrary linear order output
 -- apparently some `BEq` bug
-theorem ne_of_groupByValue {A : List PartialMatroid} {f: PartialMatroid → List ℕ} --[LinearOrder X]
+theorem ne_of_groupByValue {A : List PartialMatroid} {f: PartialMatroid → List Nat}
     {i j : Fin (groupByValue (A.mergeSort (f · < f ·)) f).length}
     (h : i ≠ j) {x y : PartialMatroid}
     (hx : x ∈ (groupByValue (A.mergeSort (f · < f ·)) f).get i)
@@ -89,15 +89,15 @@ theorem ne_of_groupByValue {A : List PartialMatroid} {f: PartialMatroid → List
   sorry
 
 
-lemma countAux_of_relabelling {L : List Nat} {f : ℕ → ℕ} (ha : f.Bijective):
-  countAux L = countAux (L.map f):= by
+lemma countAux_of_map {L : List Nat} {f : ℕ → ℕ} (ha : f.Bijective):
+    countAux L = countAux (L.map f):= by
   unfold countAux
   match L with
   | [] => simp
   | [a] => simp
   | a :: b :: l =>
     simp
-    have induction_h := @countAux_of_relabelling (b::l) f ha
+    have induction_h := @countAux_of_map (b::l) f ha
     by_cases hab : a = b
     · rw[hab]
       simp
@@ -109,3 +109,100 @@ lemma countAux_of_relabelling {L : List Nat} {f : ℕ → ℕ} (ha : f.Bijective
       simp
       rw[induction_h]
       simp
+
+lemma count_of_map {L : List Nat} {f : ℕ → ℕ} (ha : f.Bijective):
+    count L = count (L.map f):= by
+  unfold count
+  rw[countAux_of_map ha]
+
+
+--- sticking part for proofing count_of_sort_map
+def Sticking (L : List X) [LinearOrder X]: Prop :=
+    (check_stick L).Pairwise ( · ≠ · )
+
+
+/-Everything in check_stick is in the original list-/
+lemma check_stick_included (L : List X) [LinearOrder X] :
+    ∀ x ∈ check_stick L, x ∈ L := by
+  unfold check_stick
+  match L with
+  | [] => simp
+  | [a] => simp
+  | a :: b :: l =>
+    have induct_h := check_stick_included (b :: l)
+    by_cases hab : a = b
+    · rw[hab]
+      simp
+      simp at induct_h
+      exact induct_h
+    · simp
+      rw[if_neg hab]
+      simp at induct_h
+      simp
+      intro x hx
+      specialize induct_h x hx
+      exact
+        (Relation.reflGen_iff (fun a x => x = b ∨ x ∈ l) a x).mp (Relation.ReflGen.single induct_h)
+
+
+
+/-If L is sorted by ≤ , check_stick L is also Sorted by < -/
+lemma check_stick_sorted {L : List X} [LinearOrder X] (h : L.Sorted ( · ≤ · )) :
+    (check_stick L).Pairwise ( · < · ) := by
+  unfold check_stick
+  match L with
+  | [] => simp
+  | [a] => simp
+  | a :: b :: l =>
+    simp
+    have hbl : (b :: l).Sorted ( · ≤ · ) := by
+      unfold List.Sorted at h
+      simp at h
+      refine List.sorted_cons.mpr ?_
+      obtain ⟨h1, h2, h3⟩ := h
+      unfold List.Sorted
+      exact ⟨h2, h3⟩
+    have induct_h := check_stick_sorted hbl
+    by_cases hab : a = b
+    · rw[hab]
+      simp
+      exact induct_h
+    · rw [if_neg hab]
+      simp
+      constructor
+      · intro x hx
+        have h_le := check_stick_included (b :: l)
+        specialize h_le x hx
+        unfold List.Sorted at h
+        simp at h
+        obtain ⟨ h1, h2⟩ := h
+        simp at h_le
+        have hbx : b ≤ x := by
+          cases h_le with
+          | inl hxb =>
+            exact Eq.ge hxb
+          | inr hxl =>
+            obtain ⟨ h3, h4 ⟩ := h2
+            specialize h3 x hxl
+            exact h3
+        obtain ⟨ h_a_le_b, dummy⟩ := h1
+        exact lt_of_lt_of_le (lt_of_le_of_ne h_a_le_b hab) hbx
+      · apply induct_h
+
+
+lemma sort_stick (L : List X) [LinearOrder X]:
+    Sticking (L.sort) := by
+  unfold Sticking
+  -- have h := check_stick_sorted L
+  --probabily need to change L.sort into ≤, because I need to use L.sort (<) is Sorted (≤) here
+  --proof is simple, just need syntax to change < to ≠
+  sorry
+
+
+lemma count_of_sort_map {L : List (List ℕ)} {f : ℕ → ℕ} (ha : f.Bijective) :
+    count (List.sort (List.join (List.map (List.map f) L))) = count (List.sort (List.join L)) := by
+  rw [← List.map_join]
+  -- unfold count
+  -- simp [-List.map_join]
+  -- congr! 3
+  sorry
